theories/coneris/examples/hash/con_hash_interface0.v
@@ -31,6 +31,8 @@ Class con_hash0 `{!conerisGS Σ} (val_size:nat):= Con_Hash0
     Timeless (hash_tape0 α ns); 
   #[global] con_hash_view_timeless v res γ ::
     Timeless (con_hash_view0 v res γ);
+  #[global] con_hash_inv_persistent f l hm γ1 γ2 γ_lock ::
+   Persistent (con_hash_inv0 f l hm γ1 γ2 γ_lock);
   con_hash_view_frag_frag_agree k v1 v2 γ :
     con_hash_view0 k v1 γ -∗ con_hash_view0 k v2 γ -∗ ⌜v1=v2⌝; 
 
@@ -43,6 +45,17 @@ Class con_hash0 `{!conerisGS Σ} (val_size:nat):= Con_Hash0
           ↯ (ε2 n) ∗
           hash_tape0 α (ns++[fin_to_nat n]) 
       );
+
+  con_hash_init0:
+    {{{ True }}}
+      init_hash0 #()
+      {{{ (f:val), RET f; ∃ l hm γ1 γ2 γ_lock, con_hash_inv0 f l hm γ1 γ2 γ_lock }}};
+
+  con_hash_alloc_tape0:
+    {{{ True }}}
+      allocate_tape0 #()
+      {{{ (α: val), RET α; hash_tape0 α [] }}};
+  
   con_hash_spec0 f l hm γ1 γ2 γlock α n ns (v:nat):
     {{{ con_hash_inv0 f l hm γ1 γ2 γlock ∗ hash_tape0 α (n::ns) }}}
       f #v α
